theories/TLCbuffer.v
@@ -113,6 +113,198 @@ Definition eq_exec A (cmp:A->A->bool) : Prop :=
   forall x y, cmp x y = isTrue (x = y).
 
 
+
+(*----------------------*)
+(* ListAssoc *)
+
+Module LibListAssoc.
+
+
+(* ---------------------------------------------------------------------- *)
+(** ** Lookup *)
+
+Fixpoint get_opt A B (x:A) (E:list(A*B)) : option B :=
+  match E with
+  | nil => None
+  | (y,v)::E1 => If y = x
+                   then Some v
+                   else get_opt x E1
+  end.
+
+Section GetOpt.
+Variables (A B : Type).
+Implicit Types a x y : A.
+Implicit Types v : B.
+Implicit Types l : list (A*B).
+
+Lemma get_opt_nil : forall a,
+  get_opt a (nil:list(A*B)) = None.
+Proof using. auto. Qed.
+
+Lemma get_opt_cons : forall x v l a,
+  get_opt a ((x,v)::l) = (If x = a then Some v else get_opt a l).
+Proof using. auto. Qed.
+
+Lemma get_opt_app : forall l1 l2 a,
+  get_opt a (l1 ++ l2) = match get_opt a l1 with
+                         | None => get_opt a l2
+                         | Some v => Some v
+                         end.
+Proof using.
+  introv. induction l1 as [|(y,w) l1']; rew_list; simpl.
+  { auto. }
+  { case_if~. }
+Qed.
+
+End GetOpt.
+
+Hint Rewrite get_opt_nil get_opt_cons get_opt_app : rew_listx.
+
+Global Opaque get_opt.
+
+
+(* ---------------------------------------------------------------------- *)
+(** ** Equivalence *)
+
+Definition equiv A B (l1 l2:list(A*B)) :=
+  forall x, get_opt x l1 = get_opt x l2.
+
+
+(* ---------------------------------------------------------------------- *)
+(** ** Disjointness *)
+
+Definition disjoint A B (l1 l2:list(A*B)) :=
+  forall x v1 v2, get_opt x l1 = Some v1 -> get_opt x l2 = Some v2 -> False.
+
+(* TODO: equivalent definitions of disjoint using mem *)
+
+Section Disjoint.
+Variables (A B : Type).
+Implicit Types l : list (A*B).
+
+Lemma disjoint_cons_l_inv : forall x v l1 l2,
+  disjoint ((x,v)::l1) l2 ->
+  disjoint l1 l2.
+Proof using.
+  introv M. intros y v1 v2 K1 K2. tests C: (x = y).
+  { applys M v v2 K2. rewrite get_opt_cons. case_if~. }
+  { applys M v1 v2 K2. rewrite get_opt_cons. case_if~. }
+Qed.
+
+End Disjoint.
+
+
+(* ---------------------------------------------------------------------- *)
+(** ** Remove key *)
+
+Definition rem A B (x:A) (l:list(A*B)) :=
+  LibList.filter (fun '(y,v) => x <> y) l.
+
+Section Rem.
+Variables (A B : Type).
+Implicit Types a x y : A.
+Implicit Types v : B.
+Implicit Types l : list (A*B).
+
+Lemma rem_as_filter : forall a l,
+  rem a l = LibList.filter (fun '(x,v) => a <> x) l.
+Proof using. auto. Qed.
+
+Lemma rem_nil : forall a,
+  rem a (nil:list(A*B)) = nil.
+Proof using. auto. Qed.
+
+Lemma rem_cons : forall x v l a,
+  rem a ((x,v)::l) = (If x = a then rem a l else (x,v) :: rem a l).
+Proof using. intros. unfold rem. rewrite filter_cons. repeat case_if~. Qed.
+
+Lemma rem_app : forall l1 l2 a,
+  rem a (l1 ++ l2) = rem a l1 ++ rem a l2.
+Proof using. intros. unfold rem. rewrite~ filter_app. Qed.
+
+Lemma rem_last : forall x v l a,
+  rem a (l & (x,v)) = rem a l ++ (If x = a then nil else (x,v)::nil).
+Proof using. intros. unfold rem. rewrite filter_last. repeat case_if~. Qed.
+
+Lemma get_opt_rem : forall x a l,
+  get_opt x (rem a l) = (If x = a then None else get_opt x l).
+Proof using.
+  intros. induction l as [|(y,v) l']; simpl.
+  { do 2 rewrite~ get_opt_nil. case_if~. }
+  { rewrite rem_cons. rewrite get_opt_cons.
+    case_if; try rewrite get_opt_cons; repeat case_if; auto. }
+Qed.
+
+Lemma equiv_rem : forall a l1 l2,
+  equiv l1 l2 ->
+  equiv (rem a l1) (rem a l2).
+Proof using.
+  introv M. unfolds equiv. intros y.
+  do 2 rewrite get_opt_rem. case_if~.
+Qed.
+
+Lemma disjoint_rem : forall a l1 l2,
+  disjoint l1 l2 ->
+  disjoint (rem a l1) (rem a l2).
+Proof using.
+  introv D. intros y v1 v2 K1 K2. rewrite get_opt_rem in *.
+  case_if~. applys* D K1 K2.
+Qed.
+
+End Rem.
+
+Hint Rewrite rem_nil rem_cons rem_app rem_last : rew_listx.
+
+Global Opaque rem.
+
+End LibListAssoc.
+
+
+Module LibListAssocExec.
+Import LibListAssoc.
+
+Definition is_beq A (beq:A->A->bool) :=
+  forall x y, beq x y = isTrue (x = y).
+
+Fixpoint get_opt A B (beq:A->A->bool) (a:A) (l:list(A*B)) : option B :=
+  match l with
+  | nil => None
+  | (x,v)::l' => if beq x a
+                   then Some v
+                   else get_opt beq a l'
+  end.
+
+Lemma get_eq : forall A B beq a (l:list(A*B)),
+  is_beq beq ->
+  get_opt beq a l = LibListAssoc.get_opt a l.
+Proof using.
+  introv M. induction l as [|(x,v) l']; simpl.
+  { rewrite~ get_opt_nil. }
+  { rewrite~ get_opt_cons. rewrite M. repeat case_if; auto. }
+Qed.
+
+Fixpoint rem A B (beq:A->A->bool) (x:A) (E:list(A*B)) : list(A*B) :=
+  match E with
+  | nil => nil
+  | (y,v)::E' =>
+      let E'' := rem beq x E' in
+      if beq x y then E'' else (y,v)::E''
+  end.
+
+Lemma rem_eq : forall A B beq a (l:list(A*B)),
+  is_beq beq ->
+  rem beq a l = LibListAssoc.rem a l.
+Proof using.
+  introv M. induction l as [|(x,v) l']; simpl.
+  { rewrite~ rem_nil. }
+  { rewrite~ rem_cons. rewrite M. repeat case_if; fequals. }
+Qed.
+
+End LibListAssocExec.
+
+
+
+
 (*----------------------*)
 (* ListExec *)
 
